src/lowparse/LowParse.Low.Sum.fst
@@ -240,31 +240,31 @@ let finalize_sum_case
   (#kt: parser_kind)
   (#p: parser kt (sum_repr_type t))
   (s: serializer p)
-  (w: leaf_writer_strong s { kt.parser_kind_subkind == Some ParserStrong } )
+  (w: leaf_writer_strong s)
   (pc: ((x: sum_key t) -> Tot (k: parser_kind & parser k (sum_type_of_tag t x))))
   (destr: enum_repr_of_key'_t (sum_enum t))
   (k: sum_key t)
   (#rrel #rel: _)
-  (input: slice rrel rel)
+  (output: B.mbuffer byte rrel rel)
   (pos: U32.t)
 : HST.Stack unit
   (requires (fun h ->
     let len_tag = serialized_length (serialize_enum_key _ s (sum_enum t)) k in
     U32.v pos + len_tag < 4294967296 /\ (
     let pos_payload = pos `U32.add` U32.uint_to_t len_tag in
-    valid (dsnd (pc k)) h input pos_payload /\
-    writable input.base (U32.v pos) (U32.v pos_payload) h
+    bvalid (dsnd (pc k)) h output pos_payload /\
+    writable output (U32.v pos) (U32.v pos_payload) h
   )))
   (ensures (fun h _ h' ->
     let len_tag = serialized_length (serialize_enum_key _ s (sum_enum t)) k in
     let pos_payload = pos `U32.add` U32.uint_to_t len_tag in
-    B.modifies (loc_slice_from_to input pos pos_payload) h h' /\
-    valid_content_pos (parse_sum t p pc) h' input pos (synth_sum_case t k (contents (dsnd (pc k)) h input pos_payload)) (get_valid_pos (dsnd (pc k)) h input pos_payload)
+    B.modifies (B.loc_buffer_from_to output pos pos_payload) h h' /\
+    bvalid_content_pos (parse_sum t p pc) h' output pos (synth_sum_case t k (bcontents (dsnd (pc k)) h output pos_payload)) (bget_valid_pos (dsnd (pc k)) h output pos_payload)
   ))
-= let pos1 = leaf_writer_strong_to_slice_strong_prefix (write_enum_key w (sum_enum t) destr) k input pos in
+= let pos1 = (write_enum_key w (sum_enum t) destr) k output pos in
   let h = HST.get () in
   [@inline_let]
-  let _ = valid_sum_intro h t p pc input pos in
+  let _ = valid_sum_intro h t p pc (slice_of_buffer output) pos in
   ()
 
 inline_for_extraction
@@ -991,39 +991,39 @@ let finalize_dsum_case_known
   (#kt: parser_kind)
   (#p: parser kt (dsum_repr_type t))
   (s: serializer p)
-  (w: leaf_writer_strong s { kt.parser_kind_subkind == Some ParserStrong })
+  (w: leaf_writer_strong s)
   (f: ((x: dsum_known_key t) -> Tot (k: parser_kind & parser k (dsum_type_of_known_tag t x))))
   (#ku: parser_kind)
   (g: parser ku (dsum_type_of_unknown_tag t))
   (destr: enum_repr_of_key'_t (dsum_enum t))
   (k: dsum_known_key t)
   (#rrel #rel: _)
-  (input: slice rrel rel)
+  (output: B.mbuffer byte rrel rel)
   (pos: U32.t)
 : HST.Stack unit
   (requires (fun h ->
     let len_tag = serialized_length (serialize_enum_key _ s (dsum_enum t)) k in
     U32.v pos + len_tag < 4294967296 /\ (
     let pos_payload = pos `U32.add` U32.uint_to_t len_tag in
-    valid (dsnd (f k)) h input pos_payload /\
-    writable input.base (U32.v pos) (U32.v pos_payload) h
+    bvalid (dsnd (f k)) h output pos_payload /\
+    writable output (U32.v pos) (U32.v pos_payload) h
   )))
   (ensures (fun h _ h' ->
     let len_tag = serialized_length (serialize_enum_key _ s (dsum_enum t)) k in
     let pos_payload = pos `U32.add` U32.uint_to_t len_tag in
-    B.modifies (loc_slice_from_to input pos pos_payload) h h' /\
-    valid_content_pos (parse_dsum t p f g) h' input pos (synth_dsum_case t (Known k) (contents (dsnd (f k)) h input pos_payload)) (get_valid_pos (dsnd (f k)) h input pos_payload)
+    B.modifies (B.loc_buffer_from_to output pos pos_payload) h h' /\
+    bvalid_content_pos (parse_dsum t p f g) h' output pos (synth_dsum_case t (Known k) (bcontents (dsnd (f k)) h output pos_payload)) (bget_valid_pos (dsnd (f k)) h output pos_payload)
   ))
-= let pos1 = leaf_writer_strong_to_slice_strong_prefix (write_enum_key w (dsum_enum t) destr) k input pos in
+= let pos1 = (write_enum_key w (dsum_enum t) destr) k output pos in
   let h = HST.get () in
   [@inline_let]
   let _ =
-    valid_facts (parse_enum_key p (dsum_enum t)) h input pos;
-    valid_facts (parse_maybe_enum_key p (dsum_enum t)) h input pos;
-    let sq = bytes_of_slice_from h input pos in
+    bvalid_facts (parse_enum_key p (dsum_enum t)) h output pos;
+    bvalid_facts (parse_maybe_enum_key p (dsum_enum t)) h output pos;
+    let sq = bytes_of_buffer_from h output pos in
     parse_enum_key_eq p (dsum_enum t) sq;
     parse_maybe_enum_key_eq p (dsum_enum t) sq;
-    valid_dsum_intro_known h t p f g input pos
+    valid_dsum_intro_known h t p f g (slice_of_buffer output) pos
   in
   ()
 
@@ -1033,37 +1033,37 @@ let finalize_dsum_case_unknown
   (#kt: parser_kind)
   (#p: parser kt (dsum_repr_type t))
   (s: serializer p)
-  (w: leaf_writer_strong s { kt.parser_kind_subkind == Some ParserStrong })
+  (w: leaf_writer_strong s)
   (f: ((x: dsum_known_key t) -> Tot (k: parser_kind & parser k (dsum_type_of_known_tag t x))))
   (#ku: parser_kind)
   (g: parser ku (dsum_type_of_unknown_tag t))
   (r: unknown_enum_repr (dsum_enum t))
   (#rrel #rel: _)
-  (input: slice rrel rel)
+  (output: B.mbuffer byte rrel rel)
   (pos: U32.t)
 : HST.Stack unit
   (requires (fun h ->
     let len_tag = serialized_length s r in
     U32.v pos + len_tag < 4294967296 /\ (
     let pos_payload = pos `U32.add` U32.uint_to_t len_tag in
-    valid g h input pos_payload /\
-    writable input.base (U32.v pos) (U32.v pos_payload) h
+    bvalid g h output pos_payload /\
+    writable output (U32.v pos) (U32.v pos_payload) h
   )))
   (ensures (fun h _ h' ->
     let len_tag = serialized_length s r in
     let pos_payload = pos `U32.add` U32.uint_to_t len_tag in
-    B.modifies (loc_slice_from_to input pos pos_payload) h h' /\
-    valid_content_pos (parse_dsum t p f g) h' input pos (synth_dsum_case t (Unknown r) (contents g h input pos_payload)) (get_valid_pos g h input pos_payload)
+    B.modifies (B.loc_buffer_from_to output pos pos_payload) h h' /\
+    bvalid_content_pos (parse_dsum t p f g) h' output pos (synth_dsum_case t (Unknown r) (bcontents g h output pos_payload)) (bget_valid_pos g h output pos_payload)
   ))
-= let pos1 = leaf_writer_strong_to_slice_strong_prefix w r input pos in
+= let pos1 = w r output pos in
   let h = HST.get () in
   [@inline_let]
   let _ =
-    valid_facts (parse_maybe_enum_key p (dsum_enum t)) h input pos;
-    valid_facts p h input pos;
-    let sq = bytes_of_slice_from h input pos in
+    bvalid_facts (parse_maybe_enum_key p (dsum_enum t)) h output pos;
+    bvalid_facts p h output pos;
+    let sq = bytes_of_buffer_from h output pos in
     parse_maybe_enum_key_eq p (dsum_enum t) sq;
-    valid_dsum_intro_unknown h t p f g input pos
+    valid_dsum_intro_unknown h t p f g (slice_of_buffer output) pos
   in
   ()
 
